src/mem/Addresses/InfiniteAddresses.v
@@ -9,7 +9,8 @@ From Vellvm Require Import
 
 From Mem Require Import
   Addresses.MemoryAddress
-  Addresses.Provenance.
+  Addresses.Provenance
+  Tactics.
 
 From QuickChick Require Import Show.
 
@@ -21,6 +22,8 @@ From Stdlib Require Import
   Structures.Equalities.
 
 Import ListNotations.
+Import MonadNotation.
+Open Scope monad.
 
 (** ** Type of pointers
     Implementation of the notion of pointer used: an address and an offset.
@@ -94,6 +97,20 @@ Module Type Inf_HAS_POINTER_ARITHMETIC_CORE <: HAS_POINTER_ARITHMETIC_CORE InfAd
     rewrite Z.add_0_r in *.
     reflexivity.
   Qed.
+
+  Lemma ptr_add_hom :
+    forall ptr x y,
+      x >= 0 ->
+      y >= 0 ->
+      p <- ptr_add ptr x;;
+      ptr_add p y = ptr_add ptr (x + y).
+  Proof.
+    intros ptr x y X Y.
+    cbn.
+    destruct ptr; cbn; auto.
+    replace (i + x + y) with (i + (x + y)) by lia; auto.
+  Qed.
+
 End Inf_HAS_POINTER_ARITHMETIC_CORE.
 
 Module Inf_PTOI_HAS_POINTER_ARITHMETIC <: HAS_POINTER_ARITHMETIC InfAddrType := Inf_HAS_POINTER_ARITHMETIC_CORE  <+ HAS_POINTER_ARITHMETIC_HELPERS InfAddrType.
